SkLean/Preservation.lean
@@ -1,0 +1,58 @@
+/-
+# Preservation of SN and Typing Judgements
+
+In order to prove inclusion of all well-typed expressions in our reducibility candidate set, we must first prove:
+
+- That typing judgements are preserved after one-step evaluation
+- That membership in the candidate set is preserved after evaluation
+-/
+
+import SkLean.Ast
+import SkLean.Dsl
+import SkLean.Typing
+import Mathlib.Tactic
+
+/-
+## Preservation of typing judgements
+
+For unevaluable expressions, the judgement is trivially held. I define convenience lemmas for extracing the type ∀ for the left hand side of a function call and the type of the rhs.
+-/
+
+lemma match_judgement_call (ctx : Ctx) : ∀ (call : Call) (t : SkExpr), valid_judgement ctx (.call call) t → ∃ bind_ty t_body_old, valid_judgement ctx call.lhs (.fall (.mk bind_ty t_body_old)) ∧ valid_judgement ctx call.rhs bind_ty := by
+  intro c t h_judgement_t
+  cases h_judgement_t
+  case call t_lhs h_t_lhs h_t_rhs h_t =>
+    match h : t_lhs with
+      | .mk bind_ty ty_body_old =>
+        use bind_ty
+        use ty_body_old
+        simp_all
+        unfold Fall.bind_ty at h_t_rhs
+        simp at h_t_rhs
+        exact h_t_rhs
+  case beta_eq t₂ h_judgement_t₂ h_beta_eq =>
+    
+
+lemma judgement_holds_eval_once (ctx : Ctx) : ∀ (e : Call) (t : SkExpr), valid_judgement ctx (.call call) t ↔ valid_judgement ctx call.eval_once t := by
+  intro c t
+  constructor
+  intro h
+  
+  sorry
+
+lemma eval_once_candidate_iff (ctx : Ctx) : ∀ (call : Call) (t : SkExpr), is_candidate_for_t ctx (.call call) t ↔ is_candidate_for_t ctx (call.eval_once) t := by
+  intro e t
+  constructor
+  case mp =>
+    intro h
+    match h with
+      | .fn e' t' t_judgement arg h_t_arg h_redux => sorry
+      | .ty e' t' ht' =>
+        have h_judgement_t := candidate_for_t_imp_judgement_t ctx (.call e) t h
+        -- Since 
+        sorry
+      | .prp _ _ _ => sorry
+      | .fall _ _ _ => sorry
+  case mpr =>
+    intro h
+    sorry
