SkLean/Sn.lean
@@ -25,7 +25,7 @@ inductive Sn : SkExpr → Prop
   | var     (v    : Var)  : Sn (.var v)
 
 /-
-I reuse the [previous lemmas](./SnLc.lean.md) about SN bidirectionality.
+I reuse the [previous lemmas](./SnLc.lean.md) about SN bidirectionality (preservation of SN).
 -/
 
 lemma eval_rfl_imp_sn_iff : ∀ (call : Call), eval_once call = (.call call) → (Sn (eval_once call) ↔ Sn (.call call)) := by
@@ -50,3 +50,9 @@ lemma sn_bidirectional : ∀ (call : Call), Sn (eval_once call) ↔ Sn (.call ca
     exact a
   case mpr.hard a =>
     exact a
+
+/-
+We thus define our primary theorem as such. In the following chapters, I prove this statement by defining reducibility candidiates, proving all well-typed expressions are composable of reducibility candidates, and that all reducibility candidate are strongly normalizing.
+-/
+
+def all_well_typed_sn (ctx : Ctx) := ∀ (e : SkExpr) (t : SkExpr), valid_judgement ctx e t → Sn e
